\documentclass{article}
\usepackage{tikz}
\usepackage{CJKutf8}
\usepackage{amsmath}
\usepackage{amsthm}
\begin{document}
\begin{CJK}{UTF8}{gbsn}
\newtheorem*{Ex}{习题}
  \begin{Ex}
      设$A,B,C$都是集合，若$A\cup B = A\cup C$且$A\cap B = A\cap C$，试证$B=C$。
\end{Ex}
\begin{proof}[证法一]
  先证$B\subseteq C$。

  对任意的$x \in B$，分两种情况讨论：

  1)若$x \in A$:此时$x \in A\cap B$，由$A\cap B = A\cap C$知$x \in A\cap C$，从而$x \in C$。

  2)若$x \notin A$:此时由$x\in B$知$x\in A\cup B$，再由$A\cup B = A\cup C$知$x \in A\cup C$，再由$x \notin A$知$x \in C$。

  综合以上两种情况知对任意的$x$,当$x\in B$时$x\in C$，即$B \subseteq C$。
  

  由$B$和$C$的对称性知$C \subseteq B$，因此$B=C$。
\end{proof}

\begin{proof}[证法二]
  $B= B\cap (A\cup B) = B \cap (A \cup C) = (B \cap A) \cup (B \cap C) = (A \cap B) \cup (B \cap C) = (A \cap C) \cup (B \cap C) = (C \cap A) \cup (C \cap B) = C \cap (A \cup B) = C \cap (A \cup C) = C$
  
\end{proof}

\begin{proof}[证法三]
由已知条件知$(A\cup B)\setminus (A\cap B) = (A\cup C)\setminus (A\cap C)$，从而$A\bigtriangleup B = A \bigtriangleup C$，于是$A \bigtriangleup (A\bigtriangleup B) =A \bigtriangleup (A \bigtriangleup C)$, 由对称差运算的结合律知$(A \bigtriangleup A)\bigtriangleup B =(A \bigtriangleup A) \bigtriangleup C$，即$\phi \bigtriangleup B = \phi \bigtriangleup C$，从而$B = C$。
\end{proof}
\end{CJK}
\end{document}


%%% Local Variables:
%%% mode: latex
%%% TeX-master: t
%%% End:
